\documentclass[../homework.tex]{subfiles}

\pagestyle{fancy}
\fancyhf{}
\rhead{Hanzhi Zhou}
\lhead{Physics 2415 Homework}
\cfoot{\thepage}

\begin{document}
\subsection{Problem 4.1}
\subsubsection*{a)}
\begin{align*}
    F &= \int I d\vec{l} \times \vec{B} \\
      &= \int_{-\infty}^{\infty} I
      \begin{bmatrix}
          dx \\
          0 \\
          0
      \end{bmatrix} \times B_0
      \begin{bmatrix}
        e^{-\left(\frac{y}{b}\right)^2} \\
        e^{-\left(\frac{x}{a}\right)^2} \\
        0
    \end{bmatrix} \\
    &= I B_0 \int_{-\infty}^{\infty} e^{-\left(\frac{x}{a}\right)^2}\hat{k}~dx \\
    &= I B_0 a \sqrt{\pi} \hat{k}
\end{align*}

\subsubsection*{b)}
\begin{align*}
    F &= \int_{-\infty}^{\infty} I
      \begin{bmatrix}
          0 \\
          dy \\
          0
      \end{bmatrix} \times B_0
      \begin{bmatrix}
        e^{-\left(\frac{y}{b}\right)^2} \\
        e^{-\left(\frac{x}{a}\right)^2} \\
        0
    \end{bmatrix} \\
    &= I B_0 \int_{-\infty}^{\infty} -e^{-\left(\frac{y}{b}\right)^2}\hat{k}~dy \\
    &= -I B_0 b \sqrt{\pi} \hat{k}
\end{align*}

\subsubsection*{c)}
\begin{align*}
    F &= \int_{-\infty}^{\infty} I
      \begin{bmatrix}
          \cos{(\arctan{m})} dx \\
          \sin{(\arctan{m})} dy \\
          0
      \end{bmatrix} \times B_0
      \begin{bmatrix}
        e^{-\left(\frac{y}{b}\right)^2} \\
        e^{-\left(\frac{x}{a}\right)^2} \\
        0
    \end{bmatrix} \\
    &= I B_0 \int_{-\infty}^{\infty} \left(
        \frac{1}{\sqrt{1+m^2}} e^{-\left(\frac{x}{a}\right)^2} - \frac{m}{\sqrt{1+m^2}} e^{-\left(\frac{y}{b}\right)^2}
    \right)\hat{k}~dy  \\
    &= I B_0 \sqrt{\pi} \left(\frac{a}{\sqrt{1 + m^2}} - \frac{mb}{\sqrt{1 + m^2}} \right) \hat{k}
\end{align*}

\subsubsection*{d)}

\indent \indent When m = 0
\begin{equation*}
    I B_0 \sqrt{\pi} \left(\frac{a}{\sqrt{1 + 0}} - \frac{0 m}{\sqrt{1 + 0}} \right) \hat{k} = I B_0 a \sqrt{\pi} \hat{k}
\end{equation*}

When m = $\infty$, $\lim_{m \to \infty} \frac{1}{\sqrt{1+m^2}} = 0$, $\lim_{m \to \infty} \frac{m}{\sqrt{1+m^2}} = 1$
\begin{equation*}
    I B_0 \sqrt{\pi} \left(\frac{a}{\sqrt{1 + m^2}} - \frac{mb}{\sqrt{1 + m^2}} \right) \hat{k} = -I B_0 b \sqrt{\pi} \hat{k}
\end{equation*}
\end{document}